thys/LLL_Basis_Reduction/LLL.thy
@@ -63,8 +63,8 @@ abbreviation lin_indep where "lin_indep fs \<equiv> gs.lin_indpt_list (RAT fs)"
 abbreviation gso where "gso fs \<equiv> gram_schmidt_fs.gso n (RAT fs)"
 abbreviation \<mu> where "\<mu> fs \<equiv> gram_schmidt_fs.\<mu> n (RAT fs)"
 
-abbreviation reduced where "reduced fs i \<equiv> gs.reduced \<alpha> i (map (gso fs) [0..<m]) (\<mu> fs)" 
-abbreviation weakly_reduced where "weakly_reduced fs i \<equiv> gs.weakly_reduced \<alpha> i (map (gso fs) [0..<m])" 
+abbreviation reduced where "reduced fs i \<equiv> gram_schmidt_fs.reduced n (RAT fs) \<alpha> i" 
+abbreviation weakly_reduced where "weakly_reduced fs i \<equiv> gram_schmidt_fs.weakly_reduced n (RAT fs) \<alpha> i" 
   
 text \<open>lattice of initial basis\<close>
 definition "L = lattice_of fs_init" 
@@ -107,7 +107,7 @@ proof (atomize (full), goal_cases)
     by (standard) (use assms LLL_invariant_def gs.lin_indpt_list_def in auto)
   show ?case
     using assms gs'.fs_carrier gs'.f_carrier gs'.gso_carrier
-    by (auto simp add: LLL_invariant_def gs.reduced_def)
+    by (auto simp add: LLL_invariant_def gram_schmidt_fs.reduced_def)
 qed
 
 lemma LLL_invI: assumes  
@@ -199,12 +199,12 @@ proof -
   from inv(8,10) have red: "weakly_reduced fs i" 
     and sred: "reduced fs i" by (auto)
   from red red_i i have red: "weakly_reduced fs (Suc i)" 
-    unfolding gs.weakly_reduced_def
+    unfolding gram_schmidt_fs.weakly_reduced_def
     by (intro allI impI, rename_tac ii, case_tac "Suc ii = i", auto)
   from inv(11) upw have sred_i: "\<And> j. j < i \<Longrightarrow> \<bar>\<mu> fs i j\<bar> \<le> 1 / 2" 
     unfolding \<mu>_small_def by auto
   from sred sred_i have sred: "reduced fs (Suc i)"
-    unfolding gs.reduced_def
+    unfolding gram_schmidt_fs.reduced_def
     by (intro conjI[OF red] allI impI, rename_tac ii j, case_tac "ii = i", auto)
   show "LLL_invariant True (Suc i) fs" 
     by (intro LLL_invI, insert inv red sred i, auto)
@@ -390,7 +390,8 @@ proof -
     show ?case by (rule linorder_class.linorder_cases[of x i],insert G1_G eq_part eq_rest,auto)
   qed
   hence Hs:"?G' = ?G" by (auto simp:o_def)
-  have red: "weakly_reduced fs' i" using red unfolding Hs .
+  have red: "weakly_reduced fs' i" using red using eq_fs \<open>i < m\<close>
+    unfolding gram_schmidt_fs.weakly_reduced_def by simp
   let ?Mi = "M ! i ! j"  
   have Gjn: "dim_vec (fs ! j) = n" using Fij(2) carrier_vecD by blast
   define E where "E = addrow_mat m (- ?R c) i j"
@@ -478,10 +479,10 @@ proof -
     for i' j' using mu_change[of j'] mu_no_change[of i' j']
     by auto
   have sred: "reduced fs' i"
-    unfolding gs.reduced_def 
+    unfolding gram_schmidt_fs.reduced_def 
   proof (intro conjI[OF red] impI allI, goal_cases)
     case (1 i' j)
-    with mu_no_change[of i' j] sred[unfolded gs.reduced_def, THEN conjunct2, rule_format, of i' j] i 
+    with mu_no_change[of i' j] sred[unfolded gram_schmidt_fs.reduced_def, THEN conjunct2, rule_format, of i' j] i 
     show ?case by auto
   qed
 
@@ -728,9 +729,9 @@ proof -
   have take_eq: "take (Suc i - 1 - 1) fs' = take (Suc i - 1 - 1) fs" 
     by (intro nth_equalityI, insert len len' i swap(2-), auto intro!: fs'_fs) 
   from inv have "weakly_reduced fs i" by auto
-  hence "weakly_reduced fs (i - 1)" unfolding gs.weakly_reduced_def by auto
+  hence "weakly_reduced fs (i - 1)" unfolding gram_schmidt_fs.weakly_reduced_def by auto
   hence red: "weakly_reduced fs' (i - 1)"
-    unfolding gs.weakly_reduced_def using i G2_G by simp
+    unfolding gram_schmidt_fs.weakly_reduced_def using i G2_G by simp
   have i1n: "i - 1 < m" using i by auto
   let ?R = rat_of_int
   let ?RV = "map_vec ?R"  
@@ -966,7 +967,6 @@ proof -
       by (subst prod_zero_iff, auto)
     have "rat_of_int (d fs' (Suc i)) = rat_of_int (d fs (Suc i))" 
       using d_swap_unchanged[OF len i0 i _ si fs'_def] by auto
-    find_theorems name: of_int_Gramian_determinant
     also have "rat_of_int (d fs' (Suc i)) = gs.Gramian_determinant (RAT fs') (Suc i)" unfolding d_def 
       by (subst fs.of_int_Gramian_determinant[symmetric], insert conn2 i g fs', auto simp: set_conv_nth)
     also have "\<dots> = (\<Prod>j<Suc i. ?n2 j)" unfolding det2 by (rule prod.cong, insert i, auto)
@@ -1108,10 +1108,10 @@ proof -
   (* stay reduced *)
   from inv have sred: "reduced fs i" by auto
   have sred: "reduced fs' (i - 1)"
-    unfolding gs.reduced_def
+    unfolding gram_schmidt_fs.reduced_def
   proof (intro conjI[OF red] allI impI, goal_cases)
     case (1 i' j)
-    with sred have "\<bar>?mu1 i' j\<bar> \<le> 1 / 2" unfolding gs.reduced_def by auto
+    with sred have "\<bar>?mu1 i' j\<bar> \<le> 1 / 2" unfolding gram_schmidt_fs.reduced_def by auto
     thus ?case using mu'_mu_small_i[OF 1(1)] by simp
   qed
 
@@ -1265,7 +1265,7 @@ proof -
   have a1: "\<alpha> \<ge> 1" using \<alpha> by auto 
   from LLL_invD[OF LLL_inv] have
     L: "lattice_of fs = L" 
-    and red: "gs.weakly_reduced \<alpha> (length (RAT fs)) (map (gso fs) [0..<length (RAT fs)])" 
+    and red: "gram_schmidt_fs.weakly_reduced n (RAT fs) \<alpha> (length (RAT fs))" 
     and basis: "lin_indep fs" 
     and lenH: "length fs = m" 
     and H: "set fs \<subseteq> carrier_vec n" 
